added back chain's default policy
The default policies of the INPUT/OUTPUT/FORWARD chains
got lost during refactoring. We now added them back. This doesn't
change anything for the examples, since they either already have
an explicit default rule or implement everything we are verifying
without relying on the default policy.

Currently, the default policy must be specified manually. The ML
parser will be able to fill this out automatically in the future.

This commit restores the behavior documented in the FM'15 paper,
footnote 4.

Examples/Code_Interface.thy
@@ -12,22 +12,21 @@ begin
 section{*Code Interface*}
 
 (*TODO TODO TODO
-  all the unfold_ruleset_* don't add the chain's default action at the end.
-  But it should be added. This would be the responsibility of the parser.
-  How it should look like: [Rule MatchAny (Call ''FORWARD''), Rule MatchAny Drop/Allow]
+  all the unfold_ruleset_* don't add the chain's default action at the end automatically
+  This would be the responsibility of the parser.
 *)
 
-definition unfold_ruleset_FORWARD :: "common_primitive ruleset \<Rightarrow> common_primitive rule list" where
-"unfold_ruleset_FORWARD rs = ((optimize_matches opt_MatchAny_match_expr)^^10) 
-  (optimize_matches optimize_primitive_univ (rw_Reject (rm_LogEmpty (((process_call rs)^^10) [Rule MatchAny (Call ''FORWARD'')]))))"
+definition unfold_ruleset_FORWARD :: "action \<Rightarrow> common_primitive ruleset \<Rightarrow> common_primitive rule list" where
+"unfold_ruleset_FORWARD default_action rs = ((optimize_matches opt_MatchAny_match_expr)^^10) 
+  (optimize_matches optimize_primitive_univ (rw_Reject (rm_LogEmpty (((process_call rs)^^10) [Rule MatchAny (Call ''FORWARD''), Rule MatchAny default_action]))))"
 
-definition unfold_ruleset_INPUT :: "common_primitive ruleset \<Rightarrow> common_primitive rule list" where
-"unfold_ruleset_INPUT rs = ((optimize_matches opt_MatchAny_match_expr)^^10) 
-  (optimize_matches optimize_primitive_univ (rw_Reject (rm_LogEmpty (((process_call rs)^^10) [Rule MatchAny (Call ''INPUT'')]))))"
+definition unfold_ruleset_INPUT :: "action \<Rightarrow> common_primitive ruleset \<Rightarrow> common_primitive rule list" where
+"unfold_ruleset_INPUT default_action rs = ((optimize_matches opt_MatchAny_match_expr)^^10) 
+  (optimize_matches optimize_primitive_univ (rw_Reject (rm_LogEmpty (((process_call rs)^^10) [Rule MatchAny (Call ''INPUT''), Rule MatchAny default_action]))))"
 
-definition unfold_ruleset_OUTPUT :: "common_primitive ruleset \<Rightarrow> common_primitive rule list" where
-"unfold_ruleset_OUTPUT rs = ((optimize_matches opt_MatchAny_match_expr)^^10) 
-  (optimize_matches optimize_primitive_univ (rw_Reject (rm_LogEmpty (((process_call rs)^^10) [Rule MatchAny (Call ''OUTPUT'')]))))"
+definition unfold_ruleset_OUTPUT :: "action \<Rightarrow> common_primitive ruleset \<Rightarrow> common_primitive rule list" where
+"unfold_ruleset_OUTPUT default_action rs = ((optimize_matches opt_MatchAny_match_expr)^^10) 
+  (optimize_matches optimize_primitive_univ (rw_Reject (rm_LogEmpty (((process_call rs)^^10) [Rule MatchAny (Call ''OUTPUT''), Rule MatchAny default_action]))))"
 
 
 definition map_of_string :: "(string \<times> common_primitive rule list) list \<Rightarrow> string \<rightharpoonup> common_primitive rule list" where
