Examples/TUM_Net_Firewall/TUM_Spoofing.thy
@@ -78,7 +78,7 @@ open Test;
 
 declare[[ML_print_depth=50]]
 ML{*
-val rules = unfold_ruleset_FORWARD (map_of_string firewall_chains)
+val rules = unfold_ruleset_FORWARD Accept (map_of_string firewall_chains)
 *}
 ML{*
 length rules;
@@ -90,7 +90,7 @@ length lower;*}
 text{*How long does the unfolding take?*}
 ML_val{*
 val t0 = Time.now();
-val _ = unfold_ruleset_FORWARD (map_of_string firewall_chains);
+val _ = unfold_ruleset_FORWARD Accept (map_of_string firewall_chains);
 val t1= Time.now();
 writeln(String.concat ["It took ", Time.toString(Time.-(t1,t0)), " seconds"])
 *}
